src/LifetimePerms.v
@@ -1142,7 +1142,7 @@ Section LifetimePerms.
   (*
   (* edit so P is a when l P, possibly a when_ptr *)
   Lemma partial l P Q R :
-    P * lowned_Perms l (P * Q) R ⊨ lowned_Perms l Q R.
+    P * lowned_Perms l (P * Q) R ⊑ lowned_Perms l Q R.
   Proof.
     intros p0 (p & powned & Hp & (r1 & r2 & Hr1 & Hnlr2 & Hrelyr2 & Hguarr2 & Hr2 & Hlte' & Hf) & Hsep & Hlte).
     exists (p ** r1), r2.
@@ -1296,89 +1296,5 @@ Section LifetimePerms.
       apply Hpq; auto.
       destruct Hpo. specialize (sep_r _ _ H). cbn in sep_r. apply sep_r; auto.
   Qed.
-
-
-  Section MemoryPerms.
-    From Heapster Require Import
-      PermType
-      PermTypeProofs
-      MemoryPerms.
-
-    Context `{Hlens': Lens Si memory}.
-
-    Lemma Load' l xi yi xs rw R S :
-      lowned_Perms l R S * when_Perms l (xi :: ptr (rw, 0, eqp yi) ▷ xs) ⊢
-        load xi ⤳
-        (Ret tt : itree (sceE Ss) unit) :::
-        eqp yi ∅ (lowned_Perms l R S * when_Perms l (xi :: ptr (rw, 0, eqp yi) ▷ xs)).
-    Proof.
-      repeat intro. pstep. unfold load. rewritebisim @bind_trigger.
-      econstructor; eauto; try reflexivity.
-      destruct H as (powned & pwhen & Howned & Hwhen & Hsep & Hlte).
-      destruct Hwhen as (? & (pptr' & Hptr' & ?) & Hwhen); subst.
-      destruct xi as [? | [b o]]; try contradiction.
-      destruct Hptr' as (? & (v & ?) & ?); subst.
-      destruct H1 as (pptr & peq & Hpptr & Hpeq & Hsep' & Hlte').
-      cbn in Hpptr, Hpeq, Hwhen. subst.
-
-      destruct Howned as (r1 & r2 & Hsepr1 & Hnlr1 & Hnlr2 & Hrelyr2 & Hguarr2 & Hr2 & Hlte'' & Hf).
-
-      assert (read (lget c1) (b, o) = Some v).
-      {
-        apply Hlte in H0. cbn in H0. destruct H0 as (Hpreowned & Hprewhen & _).
-        apply Hwhen in Hprewhen. cbn in Hprewhen.
-        apply Hlte'' in Hpreowned. destruct Hpreowned as (_ & Hpreowned & _).
-        cbn in Hpreowned. apply Hlte' in Hprewhen; auto.
-        rewrite Nat.add_0_r in Hpptr.
-        destruct Hprewhen. apply Hpptr in H.
-        destruct rw; auto.
-      }
-      rewrite H. constructor; auto.
-      (* TODO: these exists are kind of weird *)
-      exists top_perm, ((r1 ** owned l r2 Hnlr2) ** when l pptr').
-      split; [| split; [| split]]; auto.
-      - cbn. auto.
-      - apply sep_conj_Perms_perm; auto.
-        + exists r1, r2, Hsepr1, Hnlr1, Hnlr2, Hrelyr2, Hguarr2.
-          split; [| split]; auto. reflexivity.
-        + apply when_perm_Perms; auto.
-          cbn. eexists. split; eauto.
-          cbn. exists pptr, top_perm. split; [| split; [| split]]; eauto.
-          apply separate_top.
-          rewrite sep_conj_perm_top.
-          etransitivity; eauto.
-          apply lte_l_sep_conj_perm.
-        + eapply separate_upwards_closed; eauto. symmetry.
-          eapply separate_upwards_closed; eauto. symmetry. auto.
-      - symmetry. apply separate_top.
-      - rewrite sep_conj_perm_commut. rewrite sep_conj_perm_top.
-        etransitivity; eauto.
-        apply sep_conj_perm_monotone; auto.
-    Qed.
-
-  (*
-  Lemma typing_when R1 R2 l P Q R S t s :
-    typing
-      P Q t s ->
-    @typing Si Ss R1 R2
-      (when_Perms l P * lowned_Perms l R S)
-      Q t s.
-  Proof.
-    repeat intro.
-    destruct H0 as (? & ? & ? & ? & ? & ?).
-    destruct H0 as (? & (? & ? & ?) & ?). subst.
-    cbn in *.
-    red in H.
-    apply H4 in H1. destruct H1 as (? & ? & ?). apply H6 in H1. cbn in H1.
-    specialize (H _ c1 c2 H0).
-    apply H4 in H5.
-    apply H4 in H1.
-
-    red in H.
-
-  Qed.
-   *)
-  End MemoryPerms.
-
 
 End LifetimePerms.
